redefine and complete uninit

theories/typing/uninit.v
@@ -1,17 +1,105 @@
+Require Import FunctionalExtensionality Equality.
 From iris.proofmode Require Import tactics.
 From lrust.util Require Import types.
-From lrust.typing Require Import mod_ty product.
+From lrust.typing Require Import product.
 From lrust.typing Require Export type.
 Set Default Proof Using "Type".
 
 Section uninit.
   Context `{!typeG Σ}.
 
-  Program Definition uninit1 : type unit :=
-    {| pt_size := 1;  pt_own _ _ vl := ⌜length vl = 1⌝%I |}.
-  Next Obligation. by iIntros. Qed.
-  Global Instance uninit1_send : Send uninit1. Proof. done. Qed.
+  Fixpoint uninit_shr n κ l := (match n with 0 => True |
+    S m => (∃v, &frac{κ} (λ q, l ↦{q} v)) ∗ uninit_shr m κ (l +ₗ 1) end)%I.
 
-  Definition uninit n : type unit := <{const ()}> (Π (hrepeat uninit1 n)).
+  Lemma upd_uninit_shr E vl n κ l : ↑lftN ⊆ E →
+    length vl = n → lft_ctx -∗ &{κ} (l ↦∗ vl) ={E}=∗ uninit_shr n κ l.
+  Proof.
+    move=> ?. move: vl l. elim n; [by iIntros|]=> ? IH [|v?]; [done|]=> > [=?].
+    rewrite heap_mapsto_vec_cons. iIntros "#LFT Bor".
+    iMod (bor_sep with "LFT Bor") as "[Head Tail]"; [done|].
+    iMod (bor_fracture (λ q, _ ↦{q} _)%I with "LFT Head") as "Head"; [done|].
+    iMod (IH with "LFT Tail") as "$"; [done|]. iModIntro. iExists v. iFrame.
+  Qed.
+
+  Program Definition uninit n : type unit := {|
+    ty_size := n;  ty_lfts := [];  ty_E := [];  ty_own _ _ vl := ⌜length vl = n⌝;
+    ty_shr _ κ _ l := uninit_shr n κ l;
+  |}%I.
+  Next Obligation.
+    move=>/= n _ ? _. elim n; [apply _|]=>/= *. apply bi.sep_persistent; apply _.
+  Qed.
+  Next Obligation. by iIntros. Qed. Next Obligation. by iIntros. Qed.
+  Next Obligation. by iIntros. Qed.
+  Next Obligation.
+    move=>/= n ? ? _ _. elim n; [by iIntros|]=> ? IH ?. iIntros "#? [One ?]".
+    iDestruct "One" as (v) "#?". iSplit.
+    { iExists v. by iApply frac_bor_shorten. } by iApply IH.
+  Qed.
+  Next Obligation.
+    move=>/= *. iIntros "#LFT #In Bor Tok".
+    iMod (bor_exists with "LFT Bor") as (vl) "Bor"; [done|].
+    iMod (bor_sep with "LFT Bor") as "[Bor Bor']"; [done|].
+    iMod (bor_persistent with "LFT Bor' Tok") as "[>%Eq Tok]"; [done|].
+    iApply step_fupdN_intro; [done|]. iIntros "!>!>".
+    iMod (upd_uninit_shr with "LFT Bor") as "$"; done.
+  Qed.
+  Next Obligation.
+    iIntros. iApply step_fupdN_intro; [done|]. iIntros "!>!>!>".
+    iExists [], 1%Qp. iSplit. { iPureIntro. apply proph_dep_unit. }
+    iSplit; [done|]. iIntros "_ !>". by iSplit.
+  Qed.
+  Next Obligation.
+    iIntros. iApply step_fupdN_intro; [done|]. iIntros "!>!>!>!>!>".
+    iExists [], 1%Qp. iSplit. { iPureIntro. apply proph_dep_unit. }
+    iSplit; [done|]. iIntros "_ !>". iFrame.
+  Qed.
+
+  Global Instance uninit_copy n : Copy (uninit n).
+  Proof.
+    split; [apply _|]=> ????? l q ? /=. move: l q. elim n=> [|? IH].
+    - move=> *. iIntros "_ _ Na $ !>". iExists 1%Qp, []. rewrite heap_mapsto_vec_nil.
+      iDestruct (na_own_acc with "Na") as "[$ ToNa]"; [solve_ndisj|].
+      do 2 (iSplit; [done|]). iIntros "Na". by iDestruct ("ToNa" with "Na") as "$".
+    - move=> ?? HF.
+      iIntros "#LFT [Bor Shr] Na [Tok Tok']". iDestruct "Bor" as (v) "Bor".
+      iMod (frac_bor_acc with "LFT Bor Tok") as (q) "[>Mt Close]"; [solve_ndisj|].
+      iMod (IH with "LFT Shr Na Tok'") as (q' vl) "[Na[Mt'[>%Eq Close']]]".
+      { move: HF. rewrite -Nat.add_1_l -Nat.add_assoc shr_locsE_shift. set_solver+. }
+      iDestruct (na_own_acc with "Na") as "[$ ToNa]".
+      { rewrite -Nat.add_1_l shr_locsE_shift. set_solver+. }
+      case (Qp_lower_bound q q')=> [q''[?[?[->->]]]]. iModIntro. iExists q'', (v :: vl).
+      rewrite heap_mapsto_vec_cons. iDestruct "Mt" as "[$ Mtr]".
+      iDestruct "Mt'" as "[$ Mtr']". iSplit. { iPureIntro. by rewrite /= Eq. }
+      iIntros "Na [Mt Mt']". iDestruct ("ToNa" with "Na") as "Na".
+      iMod ("Close" with "[$Mt $Mtr]") as "$".
+      by iMod ("Close'" with "Na [$Mt' $Mtr']") as "[$$]".
+  Qed.
+
+  Global Instance uninit_send n : Send (uninit n). Proof. done. Qed.
+  Global Instance uninit_sync n : Sync (uninit n). Proof. done. Qed.
+
+  Lemma list_sep_length {A} (xl: list A) m n :
+    length xl = m + n → ∃yl zl, xl = yl ++ zl ∧ length yl = m ∧ length zl = n.
+  Proof.
+    move: xl. elim m; [by exists [], xl|]=> ? IH [|x xl]; [done|]=> [=Eq].
+    case (IH xl Eq)=> [yl[zl[->[??]]]]. exists (x :: yl), zl.
+    split; [done|]. split; [|done]=>/=. by f_equal.
+  Qed.
+
+  Lemma uninit_plus_prod E L m n :
+    eqtype E L (const ((), ())) (const ()) (uninit (m + n)) (uninit m * uninit n).
+  Proof.
+    apply eqtype_unfold. { split; extensionality x; by [case x=> [[][]]|case x]. }
+    iIntros (?) "_!>_ /=". iSplit; [done|]. iSplit; [by iApply lft_equiv_refl|].
+    iSplit; iIntros "!> *".
+    - iSplit.
+      + iIntros (Eq). move: Eq=> /list_sep_length[wl[wl'[->[??]]]]. by iExists wl, wl'.
+      + iDestruct 1 as (??->?) "%". rewrite app_length. iPureIntro. by f_equal.
+    - iInduction m as [|m] "IH" forall (l)=>/=.
+      { rewrite left_id shift_loc_0. by iApply (bi.iff_refl True%I). }
+      rewrite -Nat.add_1_l -shift_loc_assoc_nat. iSplit.
+      + iDestruct 1 as "[$?]". by iApply "IH".
+      + iDestruct 1 as "[[$?]?]". iApply "IH". iFrame.
+  Qed.
 
 End uninit.
